new demand translation; cost specification for insert

src/BinomialHeap.v
@@ -19,8 +19,9 @@ From Equations Require Import Equations.
 
 From Coq Require Import Arith List Lia Setoid Morphisms Orders Program.
 Import ListNotations.
-From Clairvoyance Require Import Core Approx ApproxM List Misc BankersQueue Tick Demand.
+From Clairvoyance Require Import Core Approx ApproxM List ListA Misc Tick Demand.
 
+(*
 (** Interface to construct demand functions *)
 
 (* ApproxAlgebra records minimized with only the component relevant to use this interface.
@@ -52,11 +53,9 @@ Canonical AAnat : AA :=
 
 Parameter TODO : forall {A : Type}, A.
 
-Canonical AABool : AA :=
-  {| carrier := bool |}.
-
 Infix "**" := AAProd (at level 40).
 
+(*
 (* Demand functions *)
 Module Import DF.
 
@@ -146,33 +145,58 @@ Definition if_ {a b : AA} {x : a} {cond : bool}
 Proof. refine TODO. Defined.
 
 End DF.
-
-(* Encoding of operators *)
-
-Definition le_ {x y : nat} : DF (x, y) (x <=? y).
-Proof. refine TODO. Defined.
-
-Definition lt_ {x y : nat} : DF (x, y) (x <? y).
-Proof. refine TODO. Defined.
-
-Definition add1 {x : nat} : DF x (x + 1).
-Proof. refine TODO. Defined.
+*)
+*)
 
 Import DF.Notations.
 #[local] Open Scope df.
 
 (* Pure implementation *)
-Definition A := nat.
-
-Canonical AAA : AA :=
-  {| carrier := A |}.
+Notation A := nat (only parsing).
 
 Inductive Tree : Type :=
   | Node : nat -> A -> list Tree -> Tree.
 
-(* ApproximationAlgebra for Tree *)
-Canonical AATree : AA :=
-  {| carrier := Tree |}.
+Inductive TreeA : Type :=
+  | NodeA : T nat -> T A -> T (listA TreeA) -> TreeA.
+
+(*
+Canonical AA_A :=
+  {| carrier := A
+  ;  approx := A
+  ;  AA_Setoid := TODO
+  ;  AA_IsAA := TODO
+  ;  AA_IsAS := TODO
+  |}.
+*)
+
+Canonical AA_Tree :=
+  {| carrier := Tree
+  ;  approx := TreeA
+  ;  AA_Setoid := TODO
+  ;  AA_IsAA := TODO
+  ;  AA_IsAS := TODO
+  |}.
+
+Canonical AA_Bool : AA :=
+  {| carrier := bool
+  ;  approx := bool
+  ;  AA_Setoid := TODO
+  ;  AA_IsAA := TODO
+  ;  AA_IsAS := TODO
+  |}.
+
+
+(* Encoding of operators *)
+
+Definition le_ (x y : nat) : DF (x, y) (x <=? y).
+Proof. refine TODO. Defined.
+
+Definition lt_ (x y : nat) : DF (x, y) (x <? y).
+Proof. refine TODO. Defined.
+
+Definition add1 (x : nat) : DF x (x + 1).
+Proof. refine TODO. Defined.
 
 (* Encoding of Node *)
 Definition nodeD {r : AA} {s : r} {n : nat} {x : A} {ts : list Tree}
@@ -182,11 +206,22 @@ Proof. refine TODO. Defined.
 
 (* Encoding of match on Tree *)
 Definition match_Tree {a c : AA}
-    {g : c} {t : Tree} {f : Tree -> a}
+    {g : c} {t : Tree} (f : Tree -> a)
+    (CASE : DF g t)
     (NODE : forall n x ts, DF (g, n, x, ts) (f (Node n x ts)))
-  : DF (g, t) (f t) :=
+  : DF g (f t) :=
   match t with
   | Node n x ts => TODO >>> NODE n x ts
+  end.
+
+Definition if_ {G A : AA} {g : G} {b : bool} {P : bool -> A}
+    (CASE : DF g b)
+    (TRUE : DF g (P true))
+    (FALSE : DF g (P false))
+  : DF g (P b) :=
+  match b with
+  | true => TRUE
+  | false => FALSE
   end.
 
 Definition link (t1 t2 : Tree) : Tree :=
@@ -196,53 +231,38 @@ Definition link (t1 t2 : Tree) : Tree :=
     else Node (r2 + 1) v2 (t1 :: c2)
   end.
 
-Definition linkDF {t1 t2} : DF (t1, t2) (link t1 t2).
-Proof.
-  refine (
-  (TODO : DF (t1, t2) (t2, t1)) >>>
-  match_Tree (f := fun t1 => link t1 t2)
+Definition linkDF t1 t2 : DF (t1, t2) (link t1 t2) :=
+  DF.tick (
+  match_Tree (fun t1 => link t1 t2)
+    (var t1)
     (fun r1 v1 c1 =>
-  (TODO : DF (t2, r1, v1, c1) (r1, v1, c1, t2)) >>>
-  match_Tree (f := fun t2 => link _ t2)
-    (fun r2 v2 c2 => _
-  )))%df.
-  cbn.
-  refine (
-    if_ (f := fun b => if b then _ else _)
-        _
-        _
-        _).
-  - refine (TODO >>> le_).
-  - refine (nodeD _ _ _).
-    + refine (TODO >>> add1).
-    + refine TODO.
-    + refine (consD _ _).
-      * refine (nodeD _ _ _).
-        ** refine TODO.
-        ** refine TODO.
-        ** refine TODO.
-      * refine TODO.
-  - refine (nodeD _ _ _).
-    + refine (TODO >>> add1).
-    + refine TODO.
-    + refine (consD _ _).
-      * refine (nodeD _ _ _).
-        ** refine TODO.
-        ** refine TODO.
-        ** refine TODO.
-      * refine TODO.
-Defined.
+      match_Tree (fun t2 => link (Node r1 v1 c1) t2)
+        (var t2)
+        (fun r2 v2 c2 =>
+          if_ (P := fun b => if b then _ else _) (call (le_ v1 v2))
+              (nodeD (call (add1 r1)) (var v1) (consD (nodeD (var r2) (var v2) (var c2)) (var c1)))
+              (nodeD (call (add1 r2)) (var v2) (consD (nodeD (var r1) (var v1) (var c1)) (var c2))))
+    )
+  ).
 
 Record Heap : Type := MkHeap
   { trees : list Tree }.
 
-Canonical AAHeap : AA :=
-  {| carrier := Heap |}.
+Record HeapA : Type := MkHeapA
+  { treesA : T (listA TreeA) }.
 
-Definition MkHeapD (ts : list Tree) : DF ts (MkHeap ts).
+Canonical AA_Heap : AA :=
+  {| carrier := Heap
+  ;  approx := HeapA
+  ;  AA_Setoid := TODO
+  ;  AA_IsAA := TODO
+  ;  AA_IsAS := TODO
+  |}.
+
+Definition MkHeapD {G : AA} {ts : list Tree} {g : G} (f : DF g ts) : DF g (MkHeap ts).
 Proof. refine TODO. Defined.
 
-Definition treesD {h : Heap} : DF h (trees h).
+Definition treesD {G : AA} {g : G} {h : Heap} (f : DF g h) : DF g (trees h).
 Proof. refine TODO. Defined.
 
 Definition match_Heap {a c : AA}
@@ -258,69 +278,238 @@ Definition rank (t : Tree) : nat :=
   | (Node r v c) => r
   end.
 
-Definition rankDF {t} : DF t (rank t).
-Proof.
-  refine (TODO >>> match_Tree (f := fun t => rank t) (g := t) (*TODO*)
-    (fun r1 v1 c1 => _)).
-  cbn. refine TODO.
-Defined. 
+Definition rankDF t : DF t (rank t) :=
+  DF.tick (
+  match_Tree (fun t => rank t)
+    (var t)
+    (fun r v c => var r)
+  ).
 
 Definition root (t : Tree) : A :=
   match t with
   | (Node r v c) => v
   end.
 
-Definition rootDF {t} : DF t (root t).
-Proof.
-  refine (TODO >>> match_Tree (f := fun t => root t) (g := t) (*TODO*)
-    (fun r1 v1 c1 => _)).
-  cbn. refine TODO.
-Defined. 
+Definition rootDF t : DF t (root t) :=
+  DF.tick (
+  match_Tree (fun t => root t)
+    (var t)
+    (fun r v c => var v)
+  ).
 
 (*Assumes t has rank <= the rank of the first element of ts (if any).*)
-Fixpoint insTreeAux (t : Tree) (ts : list Tree) : list Tree :=
+Fixpoint insTree (t : Tree) (ts : list Tree) : list Tree :=
   match ts with
   | [] => [t]
   | t' :: ts' => if rank t <? rank t'
     then t :: ts
-    else insTreeAux (link t t') ts' (*t and t' should have the same rank*)
+    else insTree (link t t') ts' (*t and t' should have the same rank*)
   end.
 
-Fixpoint insTreeAuxDF (t : Tree) (ts : list Tree)
-  : DF (t, ts) (insTreeAux t ts).
-Proof.
-  refine (match_list (f := fun ts => insTreeAux t ts)
-    _ (fun t' ts' => _)).
-  - cbn. refine (consD id nilD).
-  - cbn [insTreeAux].
-    refine (if_ (f := fun b => if b then _ else _)
-              _ _ _).
-    + refine (TODO >>> lt_).
-    + refine (consD TODO (consD TODO TODO)).
-    + refine (letDF (TODO >>> @linkDF t t') _).
-      refine (TODO >>> insTreeAuxDF (link t t') ts').
-Defined.
+Fixpoint insTreeDF (t : Tree) (ts : list Tree)
+  : DF (t, ts) (insTree t ts) :=
+  DF.tick (
+    match_list (P := fun ts => insTree t ts) (var ts)
+      (consD (var t) nilD)
+      (fun t' ts' =>
+        DF.let_ (call (rankDF t)) (
+        DF.let_ (call (rankDF t')) (
+        DF.let_ (call (lt_ (rank t) (rank t'))) (
+        if_ (P := fun b => if b then _ else _) (var (rank t <? rank t'))
+          (consD (var t) (consD (var t') (var ts')))
+          (DF.let_ (call (linkDF t t')) (
+           call (insTreeDF (link t t') ts')))))))
+  ).
 
-Definition insTree (t : Tree) (hp : Heap) : Heap :=
-  MkHeap (insTreeAux t (trees hp)).
-
-Definition insTreeDF {t hp} : DF (t, hp) (insTree t hp).
-Proof.
-  refine (letDF (TODO >>> @treesD hp) _).
-  refine (letDF (TODO >>> insTreeAuxDF t (trees hp)) _).
-  refine (proj2DF >>> MkHeapD _).
-Defined.
-
-Definition insert (x : A) (hp : Heap) 
+Definition insert (x : A) (hp : Heap)
   : Heap :=
-  insTree (Node 0 x []) hp.
+  MkHeap (insTree (Node 0 x []) (trees hp)).
 
-Definition insertDF {x hp} : DF (x, hp) (insert x hp).
+Definition natD {G : AA} {g : G} (n : nat) : DF g n.
+Admitted.
+
+Definition insertDF x hp : DF (x, hp) (insert x hp) :=
+  DF.let_ (nodeD (natD 0) (var x) nilD) (
+  DF.let_ (treesD (var hp)) (
+  MkHeapD (call (insTreeDF _ _)))).
+
+Class Potential (a : AA) : Type :=
+  pot : approx a -> nat.
+
+(* number of trees *)
+#[global] Instance Potential_list {a : AA} : Potential (AA_listA a) :=
+  fun ts => 3 * sizeX 0 ts.
+
+#[global] Instance Potential_Heap : Potential AA_Heap :=
+  fun h => pot (a := AA_listA AA_Tree) (treesA h).
+
+Definition valid_Trees (ts : list Tree) : Prop.
+Admitted.
+
+Definition valid_Heap (h : Heap) : Prop := valid_Trees (trees h).
+
+Definition OTick_has_cost {A' : Type} (m : nat) (u : OTick A') (pre : A' -> nat) (post : nat) :=
+  match u with
+  | None => False
+  | Some v => m + pre (Tick.val v) + Tick.cost v <= post
+  end.
+
+Definition has_cost_ {A B : AA} {a : A} {b : B}
+    (f : DF a b) (m : nat) (pre : approx A -> nat) (post : approx B -> nat) (n : nat)
+  : Prop :=
+  forall b' : approx B, b' `is_approx` b ->
+    OTick_has_cost m (apply f b') pre (n + post b').
+
+Definition has_cost {A B : AA} {a : A} {b : B}
+    (f : DF a b) (pre : approx A -> nat) (post : approx B -> nat) (n : nat)
+  : Prop :=
+  has_cost_ f 0 pre post n.
+
+Definition potplus {A B : Type} (f : A -> nat) (g : B -> nat) (xy : A * B) : nat :=
+  f (fst xy) + g (snd xy).
+
+Infix "+++" := potplus (at level 40).
+
+Definition zero {A : Type} (_ : A) : nat := 0.
+
+(* Amortized complexity of insert *)
+Definition insert_budget := 3.
+
+Class Subadditive {A : AA} (f : approx A -> nat) : Prop :=
+  { subadditive_zero : forall x, f (bottom_of x) = 0
+  ; subadditive_lub  : forall x y, f (lub x y) <= f x + f y
+  }.
+
+Lemma let_cost {A B C : AA} {a : A} {b : B} {c : C} (f : DF a b) (g : DF (a, b) c)
+    (pre : approx A -> nat) (mid : approx B -> nat) (post : approx C -> nat) (m0 m n : nat)
+    `{!Subadditive pre}
+    (_ : has_cost_ f m0 pre mid m)
+    (_ : has_cost_ g m (pre +++ mid) post n)
+  : has_cost_ (DF.let_ f g) m0 pre post n.
 Proof.
-  refine (letDF (_ : DF _ (Node 0 x [])) _).
-  - refine (nodeD TODO TODO nilD).
-  - refine (TODO >>> insTreeDF).
-Defined.
+Admitted.
+
+(*
+  f : G -> A
+
+  g : G * A -> B
+
+  n + post b'
+  >=
+  m + cost (g' b') + pre (fst (g' b')) + mid (snd (g' b'))
+  >=
+  m0 + cost (g' b') + cost (f' ...) + pre (fst (g' b')) + pre (f' ...)
+  >=
+  m0 + cost ... + pre (lub (fst (g' b')) (f' ...))
+*)
+
+Lemma tick_cost {A B : AA} {a : A} {b : B} (f : DF a b)
+    m pre post n
+  : has_cost_ f (S m) pre post n ->
+    has_cost_ (DF.tick f) m pre post n.
+Admitted.
+
+Lemma match_list_nil_cost {G A B : AA} {P : list A -> B} {g : G}
+    `{!AutoDF g []}
+    (NIL : DF g (P []))
+    (CONS : forall x ys, DF (g, x, ys) (P (x :: ys)))
+    m pre post n
+  : has_cost_ NIL m pre post n ->
+    has_cost_ (match_list (var []) NIL CONS) m pre post n.
+Admitted.
+
+Definition pot_list {A  : AA} (x : A) (xs : list A) pot0 pot_hd pot_tl : Prop
+  := forall (x' : approx A) (xs' : approx (AA_listA A)), x' `is_approx` x -> xs' `is_approx` xs ->
+      pot0 (Thunk (ConsA (Thunk x') xs')) <= pot_hd x' + pot_tl xs'.
+
+Lemma match_list_cons_cost {G A B : AA} {P : list A -> B} {g : G} (x : A) (xs : list A)
+    `{!AutoDF g (x :: xs)}
+    (NIL : DF g (P []))
+    (CONS : forall x ys, DF (g, x, ys) (P (x :: ys)))
+    m pre pot0 m' pot_hd pot_tl post n
+  : has_cost_ (var (g := g) (x :: xs)) m pre pot0 m' ->
+    pot_list x xs pot0 pot_hd pot_tl ->
+    has_cost_ (CONS x xs) m ((pre +++ pot_hd) +++ pot_tl) post n ->
+    has_cost_ (match_list (var (x :: xs)) NIL CONS) m pre post n.
+Admitted.
+
+Lemma pot_list_pot {A : AA} (x : A) (xs : list A)
+  : pot_list x xs pot (fun _ => 3) pot.
+Proof.
+  red. intros x' xs' Ax Axs; inv Axs; cbn; lia.
+Qed.
+
+Lemma consD_cost {G A : AA} {g : G} {x : A} {xs : list A}
+    (xD : DF g x) (xsD : DF g xs) m1 m2 m pre pot n
+    `{!Subadditive pre}
+  : m1 + m2 <= m ->
+    has_cost_ xD m1 pre zero 3 ->
+    has_cost_ xsD m2 pre pot n ->
+    has_cost_ (consD xD xsD) m pre pot n.
+Admitted.
+
+Lemma nilD_cost {G A : AA} (g : G) pre n
+    `{!Subadditive pre}
+  : has_cost_ (a := g) (nilD (a := A)) 0 pre pot n.
+Proof.
+Admitted.
+
+Theorem insTree_cost (t : Tree) (ts : list Tree)
+  : valid_Trees ts ->
+    has_cost_ (insTreeDF t ts) 0 (zero +++ pot) pot insert_budget.
+Proof.
+  revert t; induction ts; intros t Vts.
+  - unfold insTreeDF.
+    apply tick_cost.
+    apply match_list_nil_cost.
+    apply consD_cost with (m1 := 1) (m2 := 0).
+    + admit.
+    + admit.
+    + admit.
+    + apply nilD_cost.
+      admit.
+  - unfold insTreeDF.
+    apply tick_cost.
+    apply match_list_cons_cost with (pot0 := pot) (pot_hd := fun _ => 3) (pot_tl := pot) (m' := 1).
+    + admit.
+    + apply pot_list_pot.
+    + apply let_cost with (mid := zero) (m := 0).
+Admitted.
+
+Lemma nodeD_cost_zero {r : AA} {s : r} (n x : nat) (ts : list Tree)
+    {pre : approx r -> nat}
+    `{!Subadditive pre}
+    (nD : DF s n) (xD : DF s x) (tsD : DF s ts)
+  : has_cost_ nD 0 pre zero 0 ->
+    has_cost_ xD 0 pre zero 0 ->
+    has_cost_ tsD 0 pre zero 0 ->
+    has_cost_ (nodeD nD xD tsD) 0 pre zero 0.
+Proof.
+Admitted.
+
+Theorem insert_cost (x : A) (h : Heap)
+  : valid_Heap h ->
+    has_cost_ (insertDF x h) 0 (zero +++ pot) pot insert_budget.
+Proof.
+  intros Vh.
+  change insert_budget with (0 + insert_budget).
+  apply let_cost with (mid := zero) (m := 0); [ admit | |].
+  { apply nodeD_cost_zero.
+    + admit.
+    + admit.
+    + admit.
+    + admit. }
+  change insert_budget with (0 + insert_budget).
+  apply let_cost with (mid := zero) (m := 0); [ admit | |].
+  { admit. }
+  assert (HH : has_cost_ (insTreeDF (Node 0 x []) (trees h)) 0 (zero +++ pot) pot insert_budget).
+  { apply insTree_cost. assumption. }
+  admit.
+Admitted.
+
+(*
+Below: TODO
+*)
 
 Fixpoint mergeAux (trs1 trs2 : list Tree) : list Tree :=
   match trs1 with
@@ -331,13 +520,14 @@ Fixpoint mergeAux (trs1 trs2 : list Tree) : list Tree :=
     | t2 :: trs2' =>
       match Nat.compare (rank t1) (rank t2) with
       | Lt => t1 :: (mergeAux trs1' trsR)
-      | Eq => trees (insTree (link t1 t2) (MkHeap (mergeAux trs1' trs2')))
+      | Eq => insTree (link t1 t2) (mergeAux trs1' trs2')
       | Gt => t2 :: merge_trs1 trs2'
       end
     end in 
     merge_trs1 trs2
   end.
 
+(*
 Canonical AABComparison : AA :=
   {| carrier := comparison |}.
 
@@ -503,3 +693,4 @@ Proof.
   - refine TODO.
   - refine TODO. (*TODO*)
 Defined.
+*)
